Execute.thy
@@ -9,8 +9,8 @@ subsection \<open>(a)\<close>
 definition solve_Unif :: "constraint \<Rightarrow> (constraint_system \<times> msg_subst) list" where
   "solve_Unif c = (if \<not>(is_Variable (c_t c)) then
                      (foldr (\<lambda>u acc. let subst = msg_unify [((c_t c), u)] in
-                                              if Option.is_none subst then acc
-                                              else ([], (Option.the subst)) # acc) ((c_M c) @ (c_A c)) [])
+                                     if Option.is_none subst then acc
+                                     else ([], (Option.the subst)) # acc) ((c_M c) @ (c_A c)) [])
                    else [])"
 
 fun solve_Comp :: "constraint \<Rightarrow> (constraint_system \<times> msg_subst) list" where
@@ -22,43 +22,44 @@ fun solve_Comp :: "constraint \<Rightarrow> (constraint_system \<times> msg_subs
 | "solve_Comp _ = []"
 
 definition solve_Proj :: "constraint \<Rightarrow> (constraint_system \<times> msg_subst) list" where
-  "solve_Proj c = concat (map (\<lambda>m. case m of Pair u v \<Rightarrow> let A = c_A c in
-                                                         let M = filter (\<lambda>m'. m = m') (c_M c) in
-                                                         [([(u # v # M) | (Pair u v # A) \<rhd> (c_t c)], Variable)]
+  "solve_Proj c = concat (map (\<lambda>m. case m of Pair t1 t2 \<Rightarrow> let A = c_A c in
+                                                           let M = filter (\<lambda>m'. m \<noteq> m') (c_M c) in
+                                                           [([(t1 # t2 # M) | (Pair t1 t2 # A) \<rhd> (c_t c)], Variable)]
                                    | _ \<Rightarrow> []) (c_M c))"
 
 definition solve_Sdec :: "constraint \<Rightarrow> (constraint_system \<times> msg_subst) list" where
   "solve_Sdec c = concat (map (\<lambda>m. case m of SymEncrypt k u \<Rightarrow> let A = c_A c in
-                                                               let M = filter (\<lambda>m'. m = m') (c_M c) in
+                                                               let M = filter (\<lambda>m'. m \<noteq> m') (c_M c) in
                                                                [([(u # M) | (SymEncrypt k u # A) \<rhd> (c_t c), (c_M c) | (SymEncrypt k u # A) \<rhd> k], Variable)]
                                    | _ \<Rightarrow> []) (c_M c))"
 
 definition solve_Adec :: "constraint \<Rightarrow> (constraint_system \<times> msg_subst) list" where
   "solve_Adec c = concat (map (\<lambda>m. case m of PubKeyEncrypt \<iota> u \<Rightarrow> let A = c_A c in
-                                                                  let M = filter (\<lambda>m'. m = m') (c_M c) in
+                                                                  let M = filter (\<lambda>m'. m \<noteq> m') (c_M c) in
                                                                   [([(u # M) | (PubKeyEncrypt \<iota> u # A) \<rhd> (c_t c)], Variable)]
                                    | _ \<Rightarrow> []) (c_M c))"
 
 definition solve_Ksub :: "constraint \<Rightarrow> (constraint_system \<times> msg_subst) list" where
   "solve_Ksub c = concat (map (\<lambda>m. case m of PubKeyEncrypt (Variable x) u \<Rightarrow> let A = c_A c in
-                                                                             let M = filter (\<lambda>m'. m = m') (c_M c) in
+                                                                             let M = filter (\<lambda>m'. m \<noteq> m') (c_M c) in
                                                                              [([c_sapply (Variable(x := \<iota>)) ((PubKeyEncrypt (Variable x) u # M) | A \<rhd> (c_t c))], Variable)]
                                    | _ \<Rightarrow> []) (c_M c))"
 
-(* TOFIX: Substitution application step is missing *)
 definition solve_rer :: "constraint_system \<Rightarrow> (constraint_system \<times> msg_subst) list" where
-  "solve_rer cs = List.maps (\<lambda>c. let unif = solve_Unif c in
-                                 let comp = solve_Comp c in
-                                 let proj = solve_Proj c in
-                                 let sdec = solve_Sdec c in
-                                 let adec = solve_Adec c in
-                                 let ksub = solve_Ksub c in
-                                 (unif @ comp @ proj @ sdec @ adec @ ksub)) cs"
+  "solve_rer cs = (let single_res = List.maps (\<lambda>c. let unif = solve_Unif c in
+                                                   let comp = solve_Comp c in
+                                                   let proj = solve_Proj c in
+                                                   let sdec = solve_Sdec c in
+                                                   let adec = solve_Adec c in
+                                                   let ksub = solve_Ksub c in
+                                                   (unif @ comp @ proj @ sdec @ adec @ ksub)) cs in
+                   let \<sigma>s = map (\<lambda>(_, \<sigma>). \<sigma>) single_res in
+                   foldr (\<lambda>\<sigma> acc. map (\<lambda>(cs, \<sigma>'). (cs_sapply \<sigma> cs, \<sigma>')) acc) \<sigma>s single_res)"
 
 subsection \<open>(b)\<close>
 
 primrec map_until :: "((constraint_system \<times> msg_subst) \<Rightarrow> (constraint_system \<times> msg_subst) option) \<Rightarrow> 
-                  (constraint_system \<times> msg_subst) list \<Rightarrow> (constraint_system \<times> msg_subst) option" where
+  (constraint_system \<times> msg_subst) list \<Rightarrow> (constraint_system \<times> msg_subst) option" where
   "map_until f [] = None" 
 | "map_until f (x # xs) = (let res = f x in 
                            if Option.is_none res then (map_until f xs)
@@ -85,17 +86,170 @@ value "map_option (\<lambda>(cs, \<sigma>). (cs, map (\<lambda>v. (v, \<sigma> v
                  [SymEncrypt (Variable ''K1'') (Constant ''m1''), PubKeyEncrypt (Variable ''B0'') (Pair (Constant ''k0'') (Sig (Variable ''A0'') (Constant ''k0''))), Constant ''a'', Constant ''b'', \<iota>] | [] \<rhd> (SymEncrypt (Constant ''k0'') (Variable ''Z0'')),
                  [SymEncrypt (Variable ''K1'') (Constant ''m1''), PubKeyEncrypt (Variable ''B0'') (Pair (Constant ''k0'') (Sig (Variable ''A0'') (Constant ''k0''))), Constant ''a'', Constant ''b'', \<iota>] | [] \<rhd> (Pair (Variable ''K1'') (Constant ''m1''))])"
 
-(* value "search [ [Constant ''a'', Constant ''b'', \<iota>] | [] \<rhd> (Pair (Variable ''A0'') (Variable ''B0'')), 
-              [PubKeyEncrypt (Variable ''B0'') (Pair (Constant ''na0'') (Variable ''A0'')),  Constant ''a'', Constant ''b'', \<iota>] | [] \<rhd> (PubKeyEncrypt (Constant ''b'') (Pair (Variable ''NA1'') (Constant ''a''))),
-              [PubKeyEncrypt (Constant ''a'') (Pair (Variable ''NA1'') (Constant ''nb1'')), PubKeyEncrypt (Variable ''B0'') (Pair (Constant ''na0'') (Variable ''A0'')),  Constant ''a'', Constant ''b'', \<iota>] | [] \<rhd> (PubKeyEncrypt (Variable ''A0'') (Pair (Constant ''na0'') (Variable ''NB0''))),
-              [PubKeyEncrypt (Variable ''B0'') (Variable ''NB0''), PubKeyEncrypt (Constant ''a'') (Pair (Variable ''NA1'') (Constant ''nb1'')), PubKeyEncrypt (Variable ''B0'') (Pair (Constant ''na0'') (Variable ''A0'')),  Constant ''a'', Constant ''b'', \<iota>] | [] \<rhd> (PubKeyEncrypt (Constant ''b'') (Constant ''nb1'')),
-              [PubKeyEncrypt (Variable ''B0'') (Variable ''NB0''), PubKeyEncrypt (Constant ''a'') (Pair (Variable ''NA1'') (Constant ''nb1'')), PubKeyEncrypt (Variable ''B0'') (Pair (Constant ''na0'') (Variable ''A0'')),  Constant ''a'', Constant ''b'', \<iota>] | [] \<rhd> (Pair (Variable ''NA1'') (Constant ''nb1''))]" *)
+value "map_option (\<lambda>(cs, \<sigma>). (cs, map (\<lambda>v. (v, \<sigma> v)) [''A0'', ''B0'', ''NA1'', ''NB0'']))
+       (search [ [Constant ''a'', Constant ''b'', \<iota>] | [] \<rhd> (Pair (Variable ''A0'') (Variable ''B0'')), 
+                 [PubKeyEncrypt (Variable ''B0'') (Pair (Constant ''na0'') (Variable ''A0'')),  Constant ''a'', Constant ''b'', \<iota>] | [] \<rhd> (PubKeyEncrypt (Constant ''b'') (Pair (Variable ''NA1'') (Constant ''a''))),
+                 [PubKeyEncrypt (Constant ''a'') (Pair (Variable ''NA1'') (Constant ''nb1'')), PubKeyEncrypt (Variable ''B0'') (Pair (Constant ''na0'') (Variable ''A0'')),  Constant ''a'', Constant ''b'', \<iota>] | [] \<rhd> (PubKeyEncrypt (Variable ''A0'') (Pair (Constant ''na0'') (Variable ''NB0''))),
+                 [PubKeyEncrypt (Variable ''B0'') (Variable ''NB0''), PubKeyEncrypt (Constant ''a'') (Pair (Variable ''NA1'') (Constant ''nb1'')), PubKeyEncrypt (Variable ''B0'') (Pair (Constant ''na0'') (Variable ''A0'')),  Constant ''a'', Constant ''b'', \<iota>] | [] \<rhd> (PubKeyEncrypt (Constant ''b'') (Constant ''nb1'')),
+                 [PubKeyEncrypt (Variable ''B0'') (Variable ''NB0''), PubKeyEncrypt (Constant ''a'') (Pair (Variable ''NA1'') (Constant ''nb1'')), PubKeyEncrypt (Variable ''B0'') (Pair (Constant ''na0'') (Variable ''A0'')),  Constant ''a'', Constant ''b'', \<iota>] | [] \<rhd> (Pair (Variable ''NA1'') (Constant ''nb1''))])"
 
 section \<open>Assignment 9\<close>
 
 subsection \<open>(a)\<close>
 
+lemma inv_Unif:
+  assumes "c = (M | A \<rhd> t)"
+    and "c \<leadsto>\<^sub>1[\<sigma>] []"
+  shows "\<exists>u. \<not>(is_Variable t) \<and> u \<in> (set M) \<union> (set A) \<and> Some(\<sigma>) = msg_unify [(t, u)]"
+  using assms(2,1)
+proof(cases rule: rer1.cases)
+  case (Unif t u M A)
+  then show ?thesis
+    using assms by auto
+qed
+
+lemma solve_Unif_sound: 
+  assumes "c = (M | A \<rhd> t)"
+    and "solve_Unif (c) = [([], \<sigma>)]"
+  shows "c \<leadsto>\<^sub>1[\<sigma>] []"
+  using assms 
+  unfolding solve_Unif_def
+  apply (simp only: Let_def)
+  sorry
+
+lemma solve_Comp_Hash_sound: 
+  assumes "c = (M | A \<rhd> (Hash t))"
+    and "\<sigma> = Variable"
+    and "cs = [(M | A \<rhd> t)]"
+    and "solve_Comp (c) = [(cs, \<sigma>)]"
+  shows "c \<leadsto>\<^sub>1[\<sigma>] cs"
+  using assms rer1.CompHash by simp
+
+lemma solve_Comp_Pair_sound: 
+  assumes "c = (M | A \<rhd> (Pair t1 t2))"
+    and "\<sigma> = Variable"
+    and "cs = [M | A \<rhd> t1, M | A \<rhd> t2]"
+    and "solve_Comp (c) = [(cs, \<sigma>)]"
+  shows "c \<leadsto>\<^sub>1[\<sigma>] cs"
+  using assms rer1.CompPair by simp
+
+lemma solve_Comp_SymEncrypt_sound: 
+  assumes "c = (M | A \<rhd> (SymEncrypt k t))"
+    and "\<sigma> = Variable"
+    and "cs = [M | A \<rhd> k, M | A \<rhd> t]"
+    and "solve_Comp (c) = [(cs, \<sigma>)]"
+  shows "c \<leadsto>\<^sub>1[\<sigma>] cs"
+  using assms rer1.CompSymEncrypt by simp
+
+lemma solve_Comp_PubKeyEncrypt_sound: 
+  assumes "c = (M | A \<rhd> (PubKeyEncrypt k t))"
+    and "\<sigma> = Variable"
+    and "cs = [M | A \<rhd> k, M | A \<rhd> t]"
+    and "solve_Comp (c) = [(cs, \<sigma>)]"
+  shows "c \<leadsto>\<^sub>1[\<sigma>] cs"
+  using assms rer1.CompPubKeyEncrypt by simp
+
+lemma solve_Comp_Sig_sound: 
+  assumes "c = (M | A \<rhd> (Sig \<iota> t))"
+    and "\<sigma> = Variable"
+    and "cs = [M | A \<rhd> \<iota>, M | A \<rhd> t]"
+    and "solve_Comp (c) = [(cs, \<sigma>)]"
+  shows "c \<leadsto>\<^sub>1[\<sigma>] cs"
+  using assms rer1.CompSig by simp
+
 subsection \<open>(b)\<close>
-(* Focus on completeness (applying case analysis on the inductive predicates) *)
+
+lemma solve_Unif_comp: 
+  assumes "c = (M | A \<rhd> t)"
+    and "c \<leadsto>\<^sub>1[\<sigma>] []"
+  shows "solve_Unif (c) = [([], \<sigma>)]"
+  using inv_Unif[of c M A t \<sigma>] 
+  unfolding solve_Unif_def
+  apply (simp only: Let_def)
+  sorry
+
+lemma solve_Comp_Hash_comp: 
+  assumes "c = (M | A \<rhd> (Hash t))"
+    and "\<sigma> = Variable"
+    and "cs = [(M | A \<rhd> t)]"
+    and "c \<leadsto>\<^sub>1[\<sigma>] cs"
+  shows "solve_Comp (c) = [(cs, \<sigma>)]"
+  using assms by simp
+
+lemma solve_Comp_Pair_comp: 
+  assumes "c = (M | A \<rhd> (Pair t1 t2))"
+    and "\<sigma> = Variable"
+    and "cs = [M | A \<rhd> t1, M | A \<rhd> t2]"
+    and "c \<leadsto>\<^sub>1[\<sigma>] cs"
+  shows "solve_Comp (c) = [(cs, \<sigma>)]"
+  using assms by simp
+
+lemma solve_Comp_SymEncrypt_comp: 
+  assumes "c = (M | A \<rhd> (SymEncrypt k t))"
+    and "\<sigma> = Variable"
+    and "cs = [M | A \<rhd> k, M | A \<rhd> t]"
+    and "c \<leadsto>\<^sub>1[\<sigma>] cs"
+  shows "solve_Comp (c) = [(cs, \<sigma>)]"
+  using assms by simp
+
+lemma solve_Comp_PubKeyEncrypt_comp: 
+  assumes "c = (M | A \<rhd> (PubKeyEncrypt k t))"
+    and "\<sigma> = Variable"
+    and "cs = [M | A \<rhd> k, M | A \<rhd> t]"
+    and "c \<leadsto>\<^sub>1[\<sigma>] cs"
+  shows "solve_Comp (c) = [(cs, \<sigma>)]"
+  using assms by simp
+
+lemma solve_Comp_Sig_comp: 
+  assumes "c = (M | A \<rhd> (Sig \<iota> t))"
+    and "\<sigma> = Variable"
+    and "cs = [M | A \<rhd> \<iota>, M | A \<rhd> t]"
+    and "c \<leadsto>\<^sub>1[\<sigma>] cs"
+  shows "solve_Comp (c) = [(cs, \<sigma>)]"
+  using assms by simp
+
+lemma solve_Proj_comp:
+  assumes "c = ((M1 @ (Pair t1 t2) # M2) | A \<rhd> t)"
+    and "\<sigma> = Variable"
+    and "cs = [(M1 @ (t1 # t2 # M2)) | ((Pair t1 t2) # A) \<rhd> t]"
+    and "c \<leadsto>\<^sub>1[\<sigma>] cs"
+  shows "solve_Proj (c) = [(cs, \<sigma>)]"
+  using assms
+  unfolding solve_Proj_def
+  apply (simp add: Let_def concat_def)
+  sorry
+
+lemma solve_Sdec_comp:
+  assumes "c = (M1 @ (SymEncrypt k t) # M2) | A \<rhd> t"
+    and "\<sigma> = Variable"
+    and "cs = [(M1 @ (u # M2)) | ((SymEncrypt k t) # A) \<rhd> t, (M1 @ M2) | ((SymEncrypt k t) # A) \<rhd> k]"
+    and "c \<leadsto>\<^sub>1[\<sigma>] cs"
+  shows "solve_Sdec (c) = [(cs, \<sigma>)]"
+  using assms
+  unfolding solve_Sdec_def
+  apply (simp add: Let_def concat_def)
+  sorry
+
+lemma solve_Adec_comp:
+  assumes "c = (M1 @ (PubKeyEncrypt \<iota> u) # M2) | A \<rhd> t"
+    and "\<sigma> = Variable"
+    and "cs = [(M1 @ (u # M2)) | ((PubKeyEncrypt \<iota> u) # A) \<rhd> t]"
+    and "c \<leadsto>\<^sub>1[\<sigma>] cs"
+  shows "solve_Adec (c) = [(cs, \<sigma>)]"
+  using assms
+  unfolding solve_Adec_def
+  apply (simp add: Let_def concat_def)
+  sorry
+
+lemma solve_Ksub_comp:
+  assumes "c = (M1 @ (PubKeyEncrypt (Variable x) u) # M2) | A \<rhd> t"
+    and "\<sigma> = Variable(x := \<iota>)"
+    and "cs = [c_sapply (Variable(x := \<iota>)) ((M1 @ (PubKeyEncrypt (Variable x) u) # M2) | A \<rhd> t)]"
+    and "c \<leadsto>\<^sub>1[\<sigma>] cs"
+  shows "solve_Ksub (c) = [(cs, \<sigma>)]"
+  using assms
+  unfolding solve_Ksub_def
+  apply (simp add: Let_def concat_def)
+  sorry
 
 end
